books/centaur/vl/expr.lisp
@@ -713,7 +713,12 @@ and generally makes it easier to write safe expression-processing code.</p>")
             (implies (vl-plusminus-p x)
                      (equal (car x) :vl-plusminus))
             :hints (("goal" :expand ((vl-plusminus-p x))))
-            :rule-classes :forward-chaining)))
+            :rule-classes :forward-chaining))
+   (local (defthm hidexpr-car-not-colon
+            (implies (vl-hidexpr-p x)
+                     (not (equal (car x) :colon)))
+            :hints(("Goal" :in-theory (enable vl-hidexpr-p
+                                              vl-hidindex-p))))))
 
 
 ; -----------------------------------------------------------------------------
@@ -730,6 +735,7 @@ and generally makes it easier to write safe expression-processing code.</p>")
            see especially @(see expr-tools).</p>"
     :measure (two-nats-measure (acl2-count x) 50)
     :base-case-override :vl-literal
+    :layout :tree
 
     (:vl-literal
      :base-name vl-literal
@@ -756,15 +762,14 @@ and generally makes it easier to write safe expression-processing code.</p>")
                "Captures the scoping that leads to some object in the
                 design. This captures the @('ape::bat::cat.dog[3][2][1].elf')
                 part of the example above.")
-      (part    vl-partselect-p
-               :default '(:none)
-               "Captures any subsequent part-selection once we get past all of
-                the indexing.  This captures the @('[10:0]') part of the
-                example above.")
       (indices vl-exprlist-p
                "Captures any subsequent indexing once we get to the thing
                 pointed to by @('scope').  This captures the @('[6][5]') part
                 of the example above.")
+      (part    vl-partselect-p
+               "Captures any subsequent part-selection once we get past all of
+                the indexing.  This captures the @('[10:0]') part of the
+                example above.")
       (atts    vl-atts-p
                "Any associated attributes.  BOZO where would you put such
                 attributes?"))
@@ -1131,9 +1136,9 @@ and generally makes it easier to write safe expression-processing code.</p>")
     :parents (vl-index)
     :short "Representation of a leading piece of a hierarchical reference to
             something, perhaps with associated indices."
-    :tag :vl-hidindex
     :measure (two-nats-measure (acl2-count x) 110)
     :measure-debug t
+    :layout :tree
 
     ((name    vl-hidname    "Leading name before the dot.")
      (indices vl-exprlist-p "Any associated indices."))
@@ -1152,38 +1157,50 @@ and generally makes it easier to write safe expression-processing code.</p>")
            @('vl-hidindex') whose @('name') is @('cat') and whose @('indices')
            are @('nil').</p>")
 
-  (deftagsum vl-hidexpr
+  (defflexsum vl-hidexpr
     :parents (vl-index)
     :short "Representation of a (possibly) hierarchical reference to something
             in the design.  For example: @('cat.dog[3][2][1].elf')."
     :measure (two-nats-measure (acl2-count x) 100)
     (:end
      :short "A lone identifier, or the final part of a hierarchical identifier."
-     ((name stringp :rule-classes :type-prescription)))
+     :cond (atom x)
+     :fields ((name :acc-body x :type stringp
+                    :rule-classes :type-prescription))
+     :ctor-body name)
     (:dot
+     :cond t
      :short "A single dot operation, perhaps with associated indices, that
              connects parts of a hierarchical identifier."
-     ((first vl-hidindex-p "The part before the dot and any associated indices.")
-      (rest  vl-hidexpr-p  "The part after the dot and indices."))))
+     :fields ((first :acc-body (car x) :type vl-hidindex-p
+                     :doc "The part before the dot and any associated indices.")
+              (rest :acc-body (cdr x) :type  vl-hidexpr-p
+                    :doc "The part after the dot and indices."))
+     :ctor-body (cons first rest)))
 
-  (deftagsum vl-scopeexpr
+  (defflexsum vl-scopeexpr
     :parents (vl-index)
     :short "Representation of a (possibly scoped, possibly hierarchical)
             reference to something in the design.  For example:
             @('ape::bat::cat.dog[3][2][1].elf')."
     :measure (two-nats-measure (acl2-count x) 110)
-    :base-case-override :end
-    (:end
-     :short "A scope expression that has no scoping operators.  For instance,
-             plain identifiers or hierarchical identifiers with no scopes."
-     ((hid vl-hidexpr-p)))
     (:colon
+     :cond (and (consp x)
+                (eq (car x) :colon))
      :short "Represents a single scoping operator (@('::') being applied to
              some interior scopeexpr."
-     ((first vl-scopename-p
-             "The outer scope name, e.g., @('ape')")
-      (rest  vl-scopeexpr-p
-             "The inner scope expression, e.g., @('bat::cat.dog[3][2][1].elf').")))
+     :shape (consp (cdr x))
+     :fields ((first :acc-body (cadr x) :type  vl-scopename-p
+                     :doc "The outer scope name, e.g., @('ape')")
+              (rest :acc-body (cddr x) :type  vl-scopeexpr-p
+                    :doc "The inner scope expression, e.g., @('bat::cat.dog[3][2][1].elf')."))
+     :ctor-body (cons :colon (cons first rest)))
+    (:end
+     :cond t
+     :short "A scope expression that has no scoping operators.  For instance,
+             plain identifiers or hierarchical identifiers with no scopes."
+     :fields ((hid :acc-body x :type vl-hidexpr-p))
+     :ctor-body hid)
 
     :long "<p>A <b>scope expression</b> extends a <b>hid expression</b> with
            arbitrarily many levels of scoping.  For instance, in the
@@ -1220,12 +1237,10 @@ and generally makes it easier to write safe expression-processing code.</p>")
     :measure (two-nats-measure (acl2-count x) 105)
     (:none
      :short "No part select."
-     :cond (or (atom x)
-               (eq (car x) :none))
-     :shape (and (consp x)
-                 (not (cdr x)))
+     :cond (atom x)
+     :shape (not x)
      :fields nil
-     :ctor-body '(:none))
+     :ctor-body nil)
     (:range
      :short "A typical @('[msb:lsb]') style part-select, e.g., @('[3:0]') or
              @('[1:5]')."
@@ -1269,6 +1284,7 @@ and generally makes it easier to write safe expression-processing code.</p>")
     :base-case-override :valuerange-single
     :short "A value or a range used in an @('inside') expression.  For instance,
             the @('8') or @('[16:20]') from @('a inside { 8, [16:20] }')."
+    :layout :tree
     (:valuerange-range
      :base-name vl-valuerange-range
      :short "A range of values from an @('inside') expression's set.  For
@@ -1302,6 +1318,7 @@ and generally makes it easier to write safe expression-processing code.</p>")
     :parents (vl-stream)
     :short "The slice size (or an indicator that there is no size) for a
             streaming expression."
+    :layout :tree
     (:expr
      :short "A slice size that is an expression, e.g., @('{<< 16 {a,b}}')
              has an expression slice size of @('16')."
@@ -1321,6 +1338,7 @@ and generally makes it easier to write safe expression-processing code.</p>")
     :short "A part of the stream in a streaming operator.  For instance,
             in @('{<< 16 {a, b with [0 +: size]}}'), the streamexprs are
             @('a') and @('b with [0 +: size]')."
+    :layout :tree
     ((expr  vl-expr-p
             "The expression part without the @('with').  Example: in the
              expression @('{<< 16 {a, b with [0 +: size]}}'), the exprs are
@@ -1403,6 +1421,7 @@ and generally makes it easier to write safe expression-processing code.</p>")
     :parents (vl-cast)
     :measure (two-nats-measure (acl2-count x) 10)
     :short "The new type/size/signedness/constness to cast an expression to."
+    :layout :tree
     (:type
      :short "A cast to a datatype, like @('int'(foo)')."
      ((type vl-datatype-p "The datatype to cast to.")))
@@ -1427,6 +1446,7 @@ and generally makes it easier to write safe expression-processing code.</p>")
     :measure (two-nats-measure (acl2-count x) 100)
     :parents (vl-pattern)
     :short "A key in an assignment pattern."
+    :layout :tree
     (:expr
      :short "An unambiguous array index pattern key like @('5') or @('foo +
              bar')."
@@ -1468,6 +1488,7 @@ and generally makes it easier to write safe expression-processing code.</p>")
     :parents (vl-pattern)
     :short "The (untyped) guts of an assignment pattern, e.g., @(''{1,2,3}'),
             @(''{a:1, b:2}'), or similar."
+    :layout :tree
     (:positional
      :short "A positional assignment pattern like @(''{1, 2, 3}')."
      ((vals  vl-exprlist-p
@@ -1499,6 +1520,7 @@ and generally makes it easier to write safe expression-processing code.</p>")
     (:vl-coretype
      :layout :tree
      :base-name vl-coretype
+     :hons t
      :short "A built-in SystemVerilog datatype like @('integer'), @('string'),
              @('void'), etc., or an array of such a type."
      ((name    vl-coretypename-p
@@ -1877,6 +1899,7 @@ and generally makes it easier to write safe expression-processing code.</p>")
     :measure (two-nats-measure (acl2-count x) 10)
     :elementp-of-nil nil
     :parents (vl-enum))
+
 
   ) ;; End of the huge mutual recursion.
 
@@ -2640,7 +2663,7 @@ and generally makes it easier to write safe expression-processing code.</p>")
 
 
 
-(defval *vl-plain-old-wire-type*
+(defval *vl-plain-old-logic-type*
   :parents (vl-datatype)
   :short "The @(see vl-datatype) for a plain @('wire') or @('logic') variable."
   :long "<p>It might seem weird to think of a @('wire') as having a datatype;
